# Closed Methods in Finding the root of non-linear system

## Bisection Method
1. Determine $x_m = \frac{x_l+x_u}{2}$
2. Find $f(x_l), f(x_m), f(x_u)$
3. Choose new interval (_find the interval with 2 different signs (+,-)_)

**Problem 1**

Determine the root of $3x^4 + 7x^3 - 15x^2 + 5x = 17$ between $[0,2]$. Use Bisection Method for 7 iterations.
The equation  becomes $f(x) = 3x^4 + 7x^3 - 15x^2 + 5x -17$. _17 is transposed so it became -17_

| $Count$    | $x_l$      | $x_m$      | $x_u$      | $f(x_l)$   | $f(x_m)$   | $f(x_u)$   | $New$            |
|------------|------------|------------|------------|------------|------------|------------|------------------|
| 1.         | 0          | 1          | 2          | -17        | $-17$      | 37         | [1,2]            |
| 2.         | 1          | 1.5        | 2          | -17        | $-4.43750$ | 37         | [1.5,2]          |
| 3.         | 1.5        | 1.75       | 2          | $-4.43750$ | $11.46484$ | 37         | [1.5,1.75]       |
| 4.         | 1.5        | 1.625      | 1.75       | $-4.43750$ | $2.47144$  | $11.46484$ | [1.5,1.625]      |
| 5.         | 1.5        | 1.5625     | 1.625      | $-4.43750$ | $-1.22432$ | $2.47144$  | [1.5625,1.625]   |
| 6.         | 1.5625     | 1.59375    | 1.625      | $-1.22432$ | $0.56087$  | $2.47144$  | [1.5625,1.59375] |
| 7.         | 1.5625     | 1.57813    | 1.59375    | $-1.22432$ | $-0.34681$ | $0.56087$  | [1.57813,1.59375]|

To get the root after the 7th iteration, use the formula of getting $x_m$. So, $x_m =\frac{1.57813+1.59375}{2} = 1.58594$

**First Iteration**

$x_m = \frac{x_l+x_u}{2} = \frac{0 + 2}{2} = 1$

$f(x_l) = 3(0)^4 + 7(0)^3 - 15(0)^2 + 5(0) - 17 = -17$

$f(x_m) = 3(1)^4 + 7(1)^3 - 15(1)^2 + 5(1) - 17 = -17$

$f(x_u) = 3(2)^4 + 7(2)^3 - 15(2)^2 + 5(2) - 17 = 37$


**Second Iteration**

$x_m = \frac{x_l+x_u}{2} = \frac{1 + 2}{2} = 1.5$

$f(x_l) = 3(1)^4 + 7(1)^3 - 15(1)^2 + 5(1) - 17 = -17$

$f(x_m) = 3(1.5)^4 + 7(1.5)^3 - 15(1.5)^2 + 5(1.5) - 17 = -4.43750$

$f(x_u) = 3(2)^4 + 7(2)^3 - 15(2)^2 + 5(2) - 17 = 37$

**Third Iteration**

$x_m = \frac{x_l+x_u}{2} = \frac{1.5 + 2}{2} = 1.75$

$f(x_l) = 3(1.5)^4 + 7(1.5)^3 - 15(1.5)^2 + 5(1.5) - 17 = -4.43750$

$f(x_m) = 3(1.75)^4 + 7(1.75)^3 - 15(1.75)^2 + 5(1.75) - 17 = 11.46484$

$f(x_u) = 3(2)^4 + 7(2)^3 - 15(2)^2 + 5(2) - 17 = 37$

**Fourth Iteration**

$x_m = \frac{x_l+x_u}{2} = \frac{1.5 + 1.75}{2} = 1.625$

$f(x_l) = 3(1.5)^4 + 7(1.5)^3 - 15(1.5)^2 + 5(1.5) - 17 = -4.43750$

$f(x_m) = 3(1.625)^4 + 7(1.625)^3 - 15(1.625)^2 + 5(1.625) - 17 = 2.47144$

$f(x_u) = 3(1.75)^4 + 7(1.75)^3 - 15(1.75)^2 + 5(1.75) - 17 = 11.46484$

**Fifth Iteration**

$x_m = \frac{x_l+x_u}{2} = \frac{1.5 + 1.625}{2} = 1.5625$

$f(x_l) = 3(1.5)^4 + 7(1.5)^3 - 15(1.5)^2 + 5(1.5) - 17 = -4.43750$

$f(x_m) = 3(1.5625)^4 + 7(1.5625)^3 - 15(1.5625)^2 + 5(1.5625) - 17 = -1.22432$

$f(x_u) = 3(1.625)^4 + 7(1.625)^3 - 15(1.625)^2 + 5(1.625) - 17 = 2.47144$

**Sixth Iteration**

$x_m = \frac{x_l+x_u}{2} = \frac{1.5625 + 1.625}{2} = 1.59375$

$f(x_l) = 3(1.5625)^4 + 7(1.5625)^3 - 15(1.5625)^2 + 5(1.5625) - 17 = -1.22432$

$f(x_m) = 3(1.59375)^4 + 7(1.59375)^3 - 15(1.59375)^2 + 5(1.59375) - 17 = 0.56087$

$f(x_u) = 3(1.625)^4 + 7(1.625)^3 - 15(1.625)^2 + 5(1.625) - 17 = 2.47144$

**Seventh Iteration**

$x_m = \frac{x_l+x_u}{2} = \frac{1.5625 + 1.59375}{2} = 1.57813$

$f(x_l) = 3(1.5625)^4 + 7(1.5625)^3 - 15(1.5625)^2 + 5(1.5625) - 17 = -1.22432$

$f(x_m) = 3(1.57813)^4 + 7(1.57813)^3 - 15(1.57813)^2 + 5(1.57813) - 17 = -0.34681$

$f(x_u) = 3(1.59375)^4 + 7(1.59375)^3 - 15(1.59375)^2 + 5(1.59375) - 17 = 0.56087$


**Problem 2**

Determine the root of $f(x) = x^3 - 2x - 5$ between [2,3]. Use Bisection for 5 iterations.

| $Count$    | $x_l$      | $x_m$      | $x_u$      | $f(x_l)$   | $f(x_m)$   | $f(x_u)$   | $New$            |
|------------|------------|------------|------------|------------|------------|------------|------------------|
| 1.         | 2          | 2.5        | 3          | -1         | 5.625      | 16         | [2,2.5]          |
| 2.         | 2          | 2.25       | 2.5        | -1         | 6.89063    | 5.625      | [2,2.25]         |
| 3.         | 2          | 2.125      | 2.25       | -1         | 0.34570    | 6.89063    | [2,2.125]        |
| 4.         | 2          | 2.0625     | 2.125      | -1         | 8.96289    | 0.34570    | [2,2.0625]       |
| 5.         | 2          | 2.03125    | 2.0625     | -1         | $-0.68161$ | 8.96289    | [2.03125,2.0625] |

To get the root after the 5th iteration, use the formula of getting $x_m$. So, $x_m =\frac{2.03125+2.0625}{2} = 2.046875$

**First Iteration**

$x_m = \frac{x_l+x_u}{2} = \frac{2 + 3}{2} = 1$

$f(x_l) = 2^3 - 2(2) - 5 = -1$

$f(x_m) = 2.5^3 - 2(2.5) - 5 = 5.625$

$f(x_u) = 3^3 - 2(3) - 5 = 16$

**Second Iteration**

$x_m = \frac{x_l+x_u}{2} = \frac{2 + 2.5}{2} = 2.25$

$f(x_l) = 2^3 - 2(2) - 5 = -1$

$f(x_m) = 2.25^3 - 2(2.25) - 5 = 6.89063$

$f(x_u) = 2.5^3 - 2(2.5) - 5 = 5.625$

**Third Iteration**

$x_m = \frac{x_l+x_u}{2} = \frac{2 + 2.25}{2} = 2.125$

$f(x_l) = 2^3 - 2(2) - 5 = -1$

$f(x_m) = 2.125^3 - 2(2.125) - 5 = 0.34570$

$f(x_u) = 2.25^3 - 2(2.25) - 5 = 6.89063$

**Fourth Iteration**

$x_m = \frac{x_l+x_u}{2} = \frac{2 + 2.125}{2} = 2.0625$

$f(x_l) = 2^3 - 2(2) - 5 = -1$

$f(x_m) = 2.0625^3 - 2(2.0625) - 5 = 8.96289$

$f(x_u) = 2.125^3 - 2(2.125) - 5 = 0.34570$

**Fifth Iteration**

$x_m = \frac{x_l+x_u}{2} = \frac{2 + 2.0625}{2} = 2.03125$

$f(x_l) = 2^3 - 2(2) - 5 = -1$

$f(x_m) = 2.03125^3 - 2(2.03125) - 5 = -0.68161$

$f(x_u) = 2.0625^3 - 2(2.0625) - 5 = 8.96289$

## False Position Method
1. Determine $f(x_u)$ and $f(x_l)$
2. Determine $x_m$
3. Determine $f(x_m)$
4. Choose new interval

The formula for finding $x_m$ is:
$x_m = \frac{x_l(f(x_u))-x_u(f(x_l))}{f(x_u)-f(x_l)}$

**Problem 1**

Determine the root of $3x^4 + 7x^3 - 15x^2 + 5x = 17$ between $[0,2]$. Use False Position Method for 7 iterations.
The equation  becomes $f(x) = 3x^4 + 7x^3 - 15x^2 + 5x -17$. _17 is transposed so it became -17_

| $Count$    | $x_l$      | $x_m$      | $x_u$      | $f(x_l)$   | $f(x_m)$   | $f(x_u)$   | $New$            |
|------------|------------|------------|------------|------------|------------|------------|------------------|
| 1.         | 0          | 0.62963    | 2          | -17        | -17.57963  | 37         | [0.62963,2]      |
| 2.         | 0.62963    | 1.07101    | 2          | -17.57963  | -16.30402  |            |                  |



**First Iteration**

$f(x_l) = 3(0)^4 + 7(0)^3 - 15(0)^2 + 5(0) - 17 = -17$

$f(x_u) = 3(2)^4 + 7(2)^3 - 15(2)^2 + 5(2) - 17 = 37$

$x_m = \frac{x_l(f(x_u))-x_u(f(x_l))}{f(x_u)-f(x_l)} = \frac{0(37)-2(-17)}{37-(-17)} = 0.62963$

$f(x_m) = 3(0.62963)^4 + 7(0.62963)^3 - 15(0.62963)^2 + 5(0.62963) - 17 = -17.57963$

**Second Iteration**

$f(x_l) = 3(0.62963)^4 + 7(0.62963)^3 - 15(0.62963)^2 + 5(0.62963) - 17 = -17.57963$

$f(x_u) = 3(2)^4 + 7(2)^3 - 15(2)^2 + 5(2) - 17 = 37$

$x_m = \frac{x_l(f(x_u))-x_u(f(x_l))}{f(x_u)-f(x_l)} = \frac{0.62963(37)-2(-17.57963)}{37-(-17.57963)} = 1.07101$

$f(x_m) = 3(1.07101)^4 + 7(1.07101)^3 - 15(1.07101)^2 + 5(1.07101) - 17 = -16.30402$
