---
title: "Open Methods in Finding the Root of a Non-linear System"
author: "Dan del Prado"
---

\newpage

# Newton Raphson Method
1. Determine $f'(x_n)$ - 1st derivative
2. Solve $f(x_n)$ and $f'(x_n)$
3. Solve for $x_{n+1}$ using $x_{n+1} = x_n - \frac{f(x_n)}{f'(x_n)}$

## Problem 1 - Newton Raphson Method

Determine the root of $3x^4 + 7x^3 - 15x^2 + 5x = 17$ between [0,2]. Use Newton Raphson method and perform 7 iterations. Use $x_0$ = 0.

$f(x_n) = 3x^4 + 7x^3 - 15x^2 + 5x - 17$

$f'(x_n) = 12x^3 + 21x^2 - 30x + 5$

| #          | $x_n$      | $f(x_n)$   | $f'(x_n)$   | $x_{n+1}$  |
|------------|------------|------------|------------ |------------|
| 0.         | 0          | -17        | 5           | 3.4        |
| 1.         | -3.4       | 502.6288   | 617.408     | 2.58590    |
| 2.         | 2.58590    | 150.81056  | 275.34665   | 2.03819    |
| 3.         | 2.03819    | 41.91987   | 132.69793   | 1.72229    |
| 4.         | 1.72229    | 9.27530    | 76.92883    | 1.60172    |
| 5.         | 1.60172    | 1.03604    | 60.13473    | 1.58449    |
| 6.         | 1.58449    | 0.01903    | 57.92449    | 1.58416    |
| 7.         | 1.58416    | -0.00008   | 57.88261    | 1.58416    |


$f(x_n) = 3(0)^4 + 7(0)^3 - 15(0)^2 + 5(0) - 17 = -17$

$f'(x_n) = 12(0)^3 + 21(0)^2 - 30(0) + 5 = 5$

$x_{n+1} = x_n - \frac{f(x_n)}{f'(x_n)} = 0-\frac{-17}{5} = 3.4$

$x_{n+1}$ becomes the new $x_n$ in the next iteration.

**First Iteration**

$f(x_n) = 3(3.4)^4 + 7(3.4)^3 - 15(3.4)^2 + 5(3.4) - 17 = 502.6288$

$f'(x_n) = 12(3.4)^3 + 21(3.4)^2 - 30(3.4) + 5 = 617.408$

$x_{n+1} = x_n - \frac{f(x_n)}{f'(x_n)} = 3.4-\frac{502.6288}{617.408} = 2.58590$

**Second Iteration**

$f(x_n) = 3(2.58590)^4 + 7(2.58590)^3 - 15(2.58590)^2 + 5(2.58590) - 17 = 150.81056$

$f'(x_n) = 12(2.58590)^3 + 21(2.58590)^2 - 30(2.58590) + 5 = 275.34665$

$x_{n+1} = x_n - \frac{f(x_n)}{f'(x_n)} = 2.58590-\frac{150.81056}{275.34665} = 2.03819$

**Third Iteration**

$f(x_n) = 3(2.03819)^4 + 7(2.03819)^3 - 15(2.03819)^2 + 5(2.03819) - 17 = 41.91987$

$f'(x_n) = 12(2.03819)^3 + 21(2.03819)^2 - 30(2.03819) + 5 = 132.69793$

$x_{n+1} = x_n - \frac{f(x_n)}{f'(x_n)} = 2.03819-\frac{41.91987}{132.69793} = 1.72229$

**Fourth Iteration**

$f(x_n) = 3(1.72229)^4 + 7(1.72229)^3 - 15(1.72229)^2 + 5(1.72229) - 17 = 9.27530$

$f'(x_n) = 12(1.72229)^3 + 21(1.72229)^2 - 30(1.72229) + 5 = 76.92883$

$x_{n+1} = x_n - \frac{f(x_n)}{f'(x_n)} = 1.72229-\frac{9.27530}{76.92883} = 1.60172$

**Fifth Iteration**

$f(x_n) = 3(1.60172)^4 + 7(1.60172)^3 - 15(1.60172)^2 + 5(1.60172) - 17 = 1.03604$

$f'(x_n) = 12(1.60172)^3 + 21(1.60172)^2 - 30(1.60172) + 5 = 60.13473$

$x_{n+1} = x_n - \frac{f(x_n)}{f'(x_n)} = 1.60172-\frac{1.03604}{60.13473} = 1.58449$

**Sixth Iteration**

$f(x_n) = 3(1.58449)^4 + 7(1.58449)^3 - 15(1.58449)^2 + 5(1.58449) - 17 = 0.01903$

$f'(x_n) = 12(1.58449)^3 + 21(1.58449)^2 - 30(1.58449) + 5 = 57.92449$

$x_{n+1} = x_n - \frac{f(x_n)}{f'(x_n)} = 1.58449-\frac{0.01903}{57.92449} = 1.58416$

**Seventh Iteration**

$f(x_n) = 3(1.58416)^4 + 7(1.58416)^3 - 15(1.58416)^2 + 5(1.58416) - 17 = -0.00008$

$f'(x_n) = 12(1.58416)^3 + 21(1.58416)^2 - 30(1.58416) + 5 = 57.88261$

$x_{n+1} = x_n - \frac{f(x_n)}{f'(x_n)} = 1.58416-\frac{-0.00008}{57.88261} = 1.58416$

## Problem 2 - Newton Raphson Method

Determine the root of $f_x = x^3 - 2x -5$ between [2,3]. Newton Raphson Method and perorm 5 iterations. Use $x_0$ = 0

$f(x_n) = x^3 - 2x - 5$

$f'(x_n) = 3x^2 - 2$

| #          | $x_n$      | $f(x_n)$   | $f'(x_n)$   | $x_{n+1}$  |
|------------|------------|------------|------------ |------------|
| 0.         | 0          | -5         | -2          | -2.5       |
| 1.         | -2.5       | 15.626     | 16.75       | -1.56716   |
| 2.         | 1.56716    | -5.71461   | 5.36797     | -0.50258   |
| 3.         | -0.50258   | -4.12179   | 1.24224     | 2.81545    |
| 4.         | 2.81545    | 11.68649   | 21.78028    | 2.27889    |
| 5.         | 2.27889    | 2.27727    | 13.58002    | 2.11120    |

$f(x_n) = 0^3 - 2(0) - 5 = -5$

$f'(x_n) = 3(0)^2 - 2 = -2$

$x_{n+1} = x_n - \frac{f(x_n)}{f'(x_n)} = 0-\frac{-5}{-2} = -2.5$

$x_{n+1}$ becomes the new $x_n$ in the next iteration.

**First Iteration**

$f(x_n) = -2.5^3 - 2(-2.5) - 5 = 15.625$

$f'(x_n) = 3(-2.5)^2 - 2 = 16.75$

$x_{n+1} = x_n - \frac{f(x_n)}{f'(x_n)} = -2.5\frac{-15.625}{16.75} = -1.56716$

**Second Iteration**

$f(x_n) = -1.56716^3 - 2(-1.56716) - 5 = -5.71461$

$f'(x_n) = 3(-1.56716)^2 - 2 = 5.36797$

$x_{n+1} = x_n - \frac{f(x_n)}{f'(x_n)} = -1.56716\frac{-5.71461}{5.36797} = -0.50258$

**Third Iteration**

$f(x_n) = -0.50258^3 - 2(-0.50258) - 5 = -4.12179$

$f'(x_n) = 3(-0.50258)^2 - 2 = 1.24224$

$x_{n+1} = x_n - \frac{f(x_n)}{f'(x_n)} = -0.50258\frac{-4.12179}{1.24224} = 2.81545$

**Fourth Iteration**

$f(x_n) = 2.81545^3 - 2(2.81545) - 5 = 11.68649$

$f'(x_n) = 3(2.81545)^2 - 2 = 21.78028$

$x_{n+1} = x_n - \frac{f(x_n)}{f'(x_n)} = 2.81545\frac{11.68649}{21.78028} = 2.27889$

**Fifth Iteration**

$f(x_n) = 2.27889^3 - 2(2.27889) - 5 = 2.27727$

$f'(x_n) = 3(2.27889)^2 - 2 = 13.58002$

$x_{n+1} = x_n - \frac{f(x_n)}{f'(x_n)} = 2.27889\frac{2.27727}{13.58002} = 2.11120$

# Secant Method
1. Solve $f(x_{n-1})$ and $f(x_n)$
2. Solve for new $x_{n+1}$ using $x_{n+1} = x_n - \frac{f(x_n)(x_n - x_{n-1}}{f(x_n)-f(x_{n-1}}$

## Problem 1 - Secant Method

Determine the root of $3x^4 + 7x^3 - 15x^2 + 5x = 17$ between [1,2]. Use Secant Method and perform 7 iterations.

| #     | $x_{n-1}$     | $x_n$     | $f(x_{n-1})$     | $f(x_n)$     | $x_{n+1}$     |
|-------|---------------|-----------|------------------|--------------|---------------|
| 0.    | 1             | 2         | -17              | 37           | 1.31481       |
| 1.    | 2             | 1.31481   | 37               | -11.48074    | 1.47707       |
| 2.    | 1.31481       | 1.47707   | -11.48074        | -5.50274     | 1.62643       |
| 3.    | 1.47707       | 1.62643   | -5.50274         | 2.56194      | 1.57898       |
| 4.    | 1.62643       | 1.57898   | 2.56194          | -0.29821     | 1.58393       |
| 5.    | 1.57898       | 1.58393   | -0.29821         | -0.01339     | 1.58416       |
| 6.    | 1.58393       | 1.58416   | -0.01339         | -0.00008     | 1.58416       |

$x_n$ is the new $x_{n-1}$ in the next iteration

$x_{n+1}$ is the new $x_n$ in the next iteration

$f(x_{n-1}) = 3(1)^4 + 7(1)^3 - 15(1)^2 + 5(1) - 17 = -17$

$f(x_n) = 3(2)^4 + 7(2)^3 - 15(2)^2 + 5(2) - 17 = 37$

$x_{n+1} = x_n - \frac{f(x_n)(x_n - x_{n-1}}{f(x_n)-f(x_{n-1}} = 2 - \frac{(37)(2-1)}{37-(-17)} = 1.31481$

**First Iteration**

$f(x_{n-1}) = 3(2)^4 + 7(2)^3 - 15(2)^2 + 5(2) - 17 = 37$

$f(x_n) = 3(1.31481)^4 + 7(1.31481)^3 - 15(1.31481)^2 + 5(1.31481) - 17 = -11.48074$

$x_{n+1} = x_n - \frac{f(x_n)(x_n - x_{n-1}}{f(x_n)-f(x_{n-1}} = 1.31481 - \frac{(-11.48074)(1.31481-2)}{-11.48074 - 37} = 1.47707$

**Second Iteration**

$f(x_{n-1}) = 3(1.31481)^4 + 7(1.31481)^3 - 15(1.31481)^2 + 5(1.31481) - 17 = -11.48074$

$f(x_n) = 3(1.47707)^4 + 7(1.47707)^3 - 15(1.47707)^2 + 5(1.47707) - 17 = -5.50274$

$x_{n+1} = x_n - \frac{f(x_n)(x_n - x_{n-1}}{f(x_n)-f(x_{n-1}} = 1.47707 - \frac{(-5.50274)(1.47707-1.31481)}{-5.50274 - (-11.48074)} = 1.62643$

**Third Iteration**

$f(x_{n-1}) = 3(1.47707)^4 + 7(1.47707)^3 - 15(1.47707)^2 + 5(1.47707) - 17 = -5.50274$

$f(x_n) = 3(1.62643)^4 + 7(1.62643)^3 - 15(1.62643)^2 + 5(1.62643) - 17 = 2.56194$

$x_{n+1} = x_n - \frac{f(x_n)(x_n - x_{n-1}}{f(x_n)-f(x_{n-1}} = 1.62643 - \frac{(2.56194)(1.62643-1.47707)}{2.56194 - (-5.50274)} = 1.57898$

**Fourth Iteration**

$f(x_{n-1}) = 3(1.62643)^4 + 7(1.62643)^3 - 15(1.62643)^2 + 5(1.62643) - 17 = 2.56194$

$f(x_n) = 3(1.57898)^4 + 7(1.57898)^3 - 15(1.57898)^2 + 5(1.57898) - 17 = -0.29821$

$x_{n+1} = x_n - \frac{f(x_n)(x_n - x_{n-1}}{f(x_n)-f(x_{n-1}} = 1.57898 - \frac{(-0.29821)(1.57898-1.62643)}{-0.29821 - 2.56194} = 1.58393$

**Fifth Iteration**

$f(x_{n-1}) = 3(1.57898)^4 + 7(1.57898)^3 - 15(1.57898)^2 + 5(1.57898) - 17 = -0.29821$

$f(x_n) = 3(1.58393)^4 + 7(1.58393)^3 - 15(1.58393)^2 + 5(1.58393) - 17 = -0.01339$

$x_{n+1} = x_n - \frac{f(x_n)(x_n - x_{n-1}}{f(x_n)-f(x_{n-1}} = 1.58393 - \frac{(-0.01339)(1.58393-1.57898)}{-0.01339 - (-0.29821)} = 1.58416$

**Sixth Iteration**

$f(x_{n-1}) = 3(1.58393)^4 + 7(1.58393)^3 - 15(1.58393)^2 + 5(1.58393) - 17 = -0.01339$

$f(x_n) = 3(1.58416)^4 + 7(1.58416)^3 - 15(1.58416)^2 + 5(1.58416) - 17 = -0.00008$

$x_{n+1} = x_n - \frac{f(x_n)(x_n - x_{n-1}}{f(x_n)-f(x_{n-1}} = 1.58416 - \frac{(-0.00008)(1.58416 - 1.58393)}{-0.00008 - (-0.01339)} = 1.58416$


## Problem 2 - Secant Method

Determine the root of $f(x) = x^3 - 2x - 5$ between [2,3]. Use the Secant Method and perform 5 iterations.

| #     | $x_{n-1}$     | $x_n$     | $f(x_{n-1})$     | $f(x_n)$     | $x_{n+1}$     |
|-------|---------------|-----------|------------------|--------------|---------------|
| 0.    | 2             | 3         | -1               | 16           | 2.05882       |
| 1.    | 3             | 2.05882   | 16               | -0.39084     | 2.08126       |
| 2.    | 2.05882       | 2.08126   | -0.39084         | -0.14724     | 2.09482       |
| 3.    | 2.08126       | 2.09482   | -0.14724         | -0.00300     | 2.09510       |
| 4.    | 2.09482       | 2.09510   | -0.0300          | -0.00612     | 2.09455       |
| 5.    | 2.09510       | 2.09455   | -0.00612         | -0.00002     | 2.09455       |

$x_n$ is the new $x_{n-1}$ in the next iteration

$x_{n+1}$ is the new $x_n$ in the next iteration

$f(x_{n-1}) = 2^3 - 2(2) - 5 = -1$

$f(x_n) = 3^3 - 2(3) - 5 = 16$

$x_{n+1} = x_n - \frac{f(x_n)(x_n - x_{n-1}}{f(x_n)-f(x_{n-1}} = 3 - \frac{(16)(3 - 2)}{16-(-1)} = 2.05882$


**First Iteration**

$f(x_{n-1}) = 3^3 - 2(3) - 5 = 16$

$f(x_n) = 2.05882^3 - 2(2.05882) - 5 = -0.39084$

$x_{n+1} = x_n - \frac{f(x_n)(x_n - x_{n-1}}{f(x_n)-f(x_{n-1}} = 2.05882 - \frac{(-0.39084)(2.05882 - 3)}{-0.39084 - 16} = 2.08126$

**Second Iteration**
$f(x_{n-1}) = 2.05882^3 - 2(2.05882) - 5 = -0.39084$

$f(x_n) = 2.08126^3 - 2(2.08126) - 5 = -0.14724$

$x_{n+1} = x_n - \frac{f(x_n)(x_n - x_{n-1}}{f(x_n)-f(x_{n-1}} = 2.08126 - \frac{(-0.14724)(2.08126 - 2.05882)}{-0.14724 - (-0.39084)} = 2.09482$

**Third Iteration**
$f(x_{n-1}) = 2.08126^3 - 2(2.08126) - 5 = -0.14724$

$f(x_n) = 2.09482^3 - 2(2.09482) - 5 = -0.00300$

$x_{n+1} = x_n - \frac{f(x_n)(x_n - x_{n-1}}{f(x_n)-f(x_{n-1}} = 2.09482 - \frac{(-0.00300)(2.09482 - 2.08126)}{-0.00300 - (-0.14724)} = 2.09510$

**Fourth Iteration**

$f(x_{n-1}) = 2.09482^3 - 2(2.09482) - 5 = -0.00300$

$f(x_n) = 2.09510^3 - 2(2.09510) - 5 = -0.00612$

$x_{n+1} = x_n - \frac{f(x_n)(x_n - x_{n-1}}{f(x_n)-f(x_{n-1}} = 2.09510 - \frac{(-0.00612)(2.09510 - 2.09482)}{-0.00612 - (-0.00300)} = 2.09455$

**Fifth Iteration**

$f(x_{n-1}) = 2.09510^3 - 2(2.09510) - 5 = -0.00612$

$f(x_n) = 2.09455^3 - 2(2.09455) - 5 = -0.00002$

$x_{n+1} = x_n - \frac{f(x_n)(x_n - x_{n-1}}{f(x_n)-f(x_{n-1}} = 2.09455 - \frac{(-0.00002)(2.09455 - 2.09510)}{-0.00002 - (-0.00612)} = 2.09455$

# Comparison of Root Values Between the 2 Methods: 

1. Problem 1
- Newton Raphson Method: 1.58416
- Secant Method: 1.58416

2. Problem 2
- Newton Raphson Method: 2.11120
- Secant Method: 2.09455
